.

LC.v
@@ -186,6 +186,172 @@ Module Helper.
     tauto.
   Qed.
 
+  Lemma fold_right_max_0_property1 :
+    forall Phi : N -> Prop,
+    (forall i : N, {Phi i} + {~ Phi i}) ->
+    forall ns : list N,
+    (forall i : N, Phi i -> In i ns) ->
+    forall n : N,
+    Phi n ->
+    fold_right max 0 ns >= n.
+  Proof.
+    intros Phi Phi_dec ns.
+    induction ns.
+    - simpl.
+      intros.
+      contradiction (H n).
+    - simpl.
+      intros.
+      assert (a >= n \/ a < n).
+        lia.
+      destruct H1.
+      * lia.
+      * cut (fold_right max 0 ns >= n).
+          lia.
+        destruct (Phi_dec n).
+        + destruct (H n p).
+          { lia.
+          }
+          { cut (
+              forall ks : list N,
+              forall k : N,
+              In k ks ->
+              fold_right max 0 ks >= k
+            ).
+              intros.
+              apply H3.
+              apply H2.
+            intros ks.
+            induction ks.
+            { simpl.
+              intros.
+              tauto.
+            }
+            { simpl.
+              intros.
+              destruct H3.
+              { subst.
+                lia.
+              }
+              { cut (fold_right Init.Nat.max 0 ks >= k).
+                  lia.
+                apply IHks.
+                apply H3.
+              }
+            }
+          }
+        + apply IHns.
+          { intros.
+            destruct (H i H2).
+            { subst.
+              contradiction n0.
+            }
+            apply H3.
+          }
+          contradiction n0.
+  Qed.
+
+  Lemma fold_right_max_0_property2 :
+    forall ns : list N,
+    forall n : N,
+    fold_right max 0 ns > n <-> (exists i : N, In i ns /\ i > n).
+  Proof.
+    intros ns.
+    induction ns.
+    - simpl.
+      intros.
+      constructor.
+      * lia.
+      * intro.
+        destruct H.
+        destruct H.
+        contradiction H.
+    - simpl.
+      intros.
+      assert (a > (fold_right Init.Nat.max 0 ns) \/ a <= (fold_right Init.Nat.max 0 ns)).
+        lia.
+      destruct H.
+      * constructor.
+        + intros.
+          exists a.
+          constructor.
+          left.
+          reflexivity.
+          lia.
+        + intros.
+          destruct H0 as [i].
+          destruct H0.
+          destruct H0.
+          subst.
+          lia.
+          assert (fold_right Init.Nat.max 0 ns > n).
+            apply IHns.
+            exists i.
+            constructor.
+            apply H0.
+            apply H1.
+          lia.
+      * constructor.
+        + intros.
+          assert (fold_right Init.Nat.max 0 ns > n).
+            lia.
+          destruct (proj1 (IHns n) H1) as [i].
+          destruct H2.
+          exists i.
+          constructor.
+          right.
+          apply H2.
+          apply H3.
+        + intros.
+          destruct H0 as [i].
+          destruct H0.
+          destruct H0.
+          subst.
+          lia.
+          assert (fold_right max 0 ns > n).
+            apply IHns.
+            exists i.
+            constructor.
+            apply H0.
+            apply H1.
+          lia.
+  Qed.
+
+  Lemma forallb_true_iff {A : Type} {Phi : A -> Bool} :
+    forall xs : list A,
+    forallb Phi xs = true <-> (forall x : A, In x xs -> Phi x = true).
+  Proof.
+    intros xs.
+    induction xs.
+    - simpl.
+      tauto.
+    - simpl.
+      constructor.
+      * intros.
+        assert (Phi a = true /\ forallb Phi xs = true).
+          apply andb_true_iff.
+          apply H.
+        destruct H1.
+        destruct H0.
+        + subst.
+          apply H1.
+        + apply IHxs.
+          apply H2.
+          apply H0.
+      * intros.
+        cut (Phi a = true /\ forallb Phi xs = true).
+          apply andb_true_iff.
+        constructor.
+        + apply H.
+          left.
+          reflexivity.
+        + apply IHxs.
+          intros.
+          apply H.
+          right.
+          apply H0.
+  Qed.
+
 End Helper.
 
 Module STLC.
@@ -204,11 +370,84 @@ Module STLC.
   | Abs : forall iv : IVar, forall tm1 : Tm, Tm
   .
 
+  Lemma Tm_eq_dec :
+    forall tm1 : Tm,
+    forall tm2 : Tm,
+    {tm1 = tm2} + {tm1 <> tm2}.
+  Proof.
+    intros tm1.
+    induction tm1.
+    - intros tm2.
+      destruct tm2.
+      * destruct (Nat.eq_dec iv iv0).
+        + left.
+          subst.
+          reflexivity.
+        + right.
+          intro.
+          inversion H.
+          contradiction n.
+      * right.
+        intro.
+        inversion H.
+      * right.
+        intro.
+        inversion H.
+    - intros tm2.
+      destruct tm2.
+      * right.
+        intro.
+        inversion H.
+      * destruct (IHtm1_1 tm2_1).
+        + subst.
+          destruct (IHtm1_2 tm2_2).
+          { subst.
+            left.
+            reflexivity.
+          }
+          { right.
+            intro.
+            inversion H.
+            contradiction n.
+          }
+        + right.
+          intro.
+          inversion H.
+          contradiction n.
+      * right.
+        intro.
+        inversion H.
+    - intros tm2.
+      destruct tm2.
+      * right.
+        intro.
+        inversion H.
+      * right.
+        intro.
+        inversion H.
+      * destruct (Nat.eq_dec iv iv0).
+        + subst.
+          destruct (IHtm1 tm2).
+          { subst.
+            left.
+            reflexivity.
+          }
+          { right.
+            intro.
+            inversion H.
+            contradiction n.
+          }
+        + right.
+          intro.
+          inversion H.
+          contradiction n.
+  Qed.
+
   Fixpoint isFreeIn (iv0 : IVar) (tm : Tm) : Bool :=
     match tm with
     | Var iv => if Nat.eq_dec iv0 iv then true else false
     | App tm1 tm2 => orb (isFreeIn iv0 tm1) (isFreeIn iv0 tm2)
-    | Abs iv tm1 => andb (isFreeIn iv0 tm1) (negb (Nat.eqb iv0 iv))
+    | Abs iv tm1 => andb (isFreeIn iv0 tm1) (if Nat.eq_dec iv0 iv then false else true)
     end
   .
 
@@ -216,241 +455,449 @@ Module STLC.
     isFreeIn iv0 tm = true
   .
 
+  Lemma FreeIn_dec :
+    forall iv0 : IVar,
+    forall tm : Tm,
+    {FreeIn iv0 tm} + {~ FreeIn iv0 tm}.
+  Proof.
+    cut (
+      forall tm : Tm,
+      forall iv0 : IVar,
+      {FreeIn iv0 tm} + {~ FreeIn iv0 tm}
+    ).
+      intros.
+      destruct (H tm iv0).
+      tauto.
+      tauto.
+    intros.
+    unfold FreeIn.
+    destruct (isFreeIn iv0 tm).
+    left.
+    reflexivity.
+    right.
+    intro.
+    inversion H.
+  Qed.
+
+  Lemma FreeIn_Var :
+    forall iv0 : IVar,
+    forall iv : IVar,
+    FreeIn iv0 (Var iv) <-> iv0 = iv.
+  Proof.
+    intros.
+    constructor.
+    - intros.
+      inversion H.
+      destruct (Nat.eq_dec iv0 iv).
+      * apply e.
+      * inversion H1.
+    - intros.
+      subst.
+      unfold FreeIn.
+      simpl.
+      destruct (Nat.eq_dec iv iv).
+      * reflexivity.
+      * contradiction n.
+        reflexivity.
+  Qed.
+
   Definition FreshIn (iv0 : IVar) (tm : Tm) : Prop :=
     isFreeIn iv0 tm = false
   .
+
+  Lemma FreshIn_iff :
+    forall iv0 : IVar,
+    forall tm : Tm,
+    FreshIn iv0 tm <-> ~ FreeIn iv0 tm.
+  Proof.
+    intros.
+    unfold FreeIn.
+    unfold FreshIn.
+    destruct (isFreeIn iv0 tm).
+    - intuition.
+    - intuition.
+  Qed.
+
+  Lemma FreshIn_dec :
+    forall iv0 : IVar,
+    forall tm : Tm,
+    {FreshIn iv0 tm} + {~ FreshIn iv0 tm}.
+  Proof.
+    intros.
+    assert (FreshIn iv0 tm <-> ~ FreeIn iv0 tm).
+      apply FreshIn_iff.
+    destruct (FreeIn_dec iv0 tm).
+    - right.
+      tauto.
+    - left.
+      tauto.
+  Qed.
+
+  Lemma FreshIn_Var :
+    forall iv0 : IVar,
+    forall iv : IVar,
+    FreshIn iv0 (Var iv) <-> iv0 <> iv.
+  Proof.
+    intros.
+    assert (FreshIn iv0 (Var iv) <-> ~ FreeIn iv0 (Var iv)).
+      apply FreshIn_iff.
+    assert (FreeIn iv0 (Var iv) <-> iv0 = iv).
+      apply FreeIn_Var.
+    tauto.
+  Qed.
+
+  Fixpoint getFVs (tm : Tm) : list IVar :=
+    match tm with
+    | Var iv => [iv]
+    | App tm1 tm2 => getFVs tm1 ++ getFVs tm2
+    | Abs iv tm1 => remove Nat.eq_dec iv (getFVs tm1)
+    end
+  .
+
+  Lemma getFVs_returns_free_vars :
+    forall iv : IVar,
+    forall tm : Tm,
+    In iv (getFVs tm) <-> FreeIn iv tm.
+  Proof.
+    cut (
+      forall tm : Tm,
+      forall iv0 : IVar,
+      In iv0 (getFVs tm) <-> FreeIn iv0 tm
+    ).
+      intros.
+      apply (H tm iv).
+    intros tm.
+    induction tm.
+    - intros.
+      constructor.
+      * intros.
+        inversion H.
+        + subst.
+          apply FreeIn_Var.
+          reflexivity.
+        + inversion H0.
+      * intros.
+        simpl.
+        left.
+        cut (iv0 = iv).
+          intuition.
+        apply FreeIn_Var.
+        apply H.
+    - intros.
+      unfold FreeIn.
+      simpl.
+      constructor.
+      * intros.
+        destruct (in_app_or _ _ _ H).
+        + apply orb_true_iff.
+          left.
+          apply IHtm1.
+          apply H0.
+        + apply orb_true_iff.
+          right.
+          apply IHtm2.
+          apply H0.
+      * intros.
+        assert (isFreeIn iv0 tm1 = true \/ isFreeIn iv0 tm2 = true).
+          apply orb_true_iff.
+          apply H.
+        destruct H0.
+        + apply in_or_app.
+          left.
+          apply IHtm1.
+          apply H0.
+        + apply in_or_app.
+          right.
+          apply IHtm2.
+          apply H0.
+    - intros.
+      unfold FreeIn.
+      simpl.
+      constructor.
+      * intro.
+        apply andb_true_iff.
+        constructor.
+        + apply IHtm.
+          apply (in_remove Nat.eq_dec _ iv0 iv).
+          apply H.
+        + destruct (Nat.eq_dec iv0 iv).
+          { subst.
+            contradiction (remove_In _ (getFVs tm) iv H).
+          }
+          { reflexivity.
+          }
+      * intro.
+        assert (isFreeIn iv0 tm = true /\ (if Nat.eq_dec iv0 iv then false else true) = true).
+          apply andb_true_iff.
+          apply H.
+        destruct H0.
+        apply in_in_remove.
+        + destruct (Nat.eq_dec iv0 iv).
+          { inversion H1.
+          }
+          { apply n.
+          }
+        + apply IHtm.
+          apply H0.
+  Qed.
 
   Definition Subst : Type :=
     list (IVar * Tm)
   .
 
-  Fixpoint substVar (sigma : Subst) (iv0 : IVar) : Tm :=
-    match sigma with
+  Fixpoint runSubst_Var (sub : Subst) (iv0 : IVar) : Tm :=
+    match sub with
     | [] => Var iv0
-    | (iv, tm) :: sigma' =>
-      if Nat.eq_dec iv0 iv
+    | (iv, tm) :: sub' =>
+      if Nat.eq_dec iv iv0
       then tm
-      else substVar sigma' iv0
+      else runSubst_Var sub' iv0
     end
   .
 
-  Lemma getFreshVariableBound :
-    forall sigma : Subst,
+  Inductive IsProperSubst : Subst -> Prop :=
+  | NilSubst :
+    IsProperSubst []
+  | ConsSubst :
+    forall iv : IVar,
     forall tm : Tm,
-    { bound : N
-    | forall iv0 : IVar,
-      iv0 > bound ->
-      forall iv : IVar,
-      FreeIn iv tm ->
-      FreshIn iv0 (substVar sigma iv)
-    }.
-  Proof.
-    assert ( claim1 :
-      forall tm : Tm,
-      { iv0 : IVar
-      | forall iv : IVar,
-        isFreeIn iv tm = true ->
-        iv0 >= iv
-      }
-    ).
-      intros tm; induction tm.
-      (* 1st *)
-        exists iv.
-        simpl.
-        intros.
-        destruct (Nat.eq_dec iv0 iv).
-        (* e : iv0 = iv *)
-        lia.
-        (* n : iv0 <> iv *)
-        inversion H.
-      (* 2nd *)
-        destruct IHtm1 as [iv1 H1].
-        destruct IHtm2 as [iv2 H2].
-        exists (max iv1 iv2).
-        simpl.
-        intros.
-        assert (isFreeIn iv tm1 = true \/ isFreeIn iv tm2 = true).
-          apply orb_true_iff.
-          apply H.
-        destruct H0.
-        (* isFreeIn iv tm1 = true *)
-        assert (iv1 >= iv).
-          apply H1.
-          apply H0.
-        lia.
-        (* isFreeIn iv tm2 = true *)
-        assert (iv2 >= iv).
-          apply H2.
-          apply H0.
-        lia.
-      (* 3rd *)
-      destruct IHtm as [iv1 H1].
-      exists iv1.
-      intros.
-      inversion H.
-      assert (isFreeIn iv0 tm = true).
-        apply (andb_true_iff _ (negb (iv0 =? iv))).
-        apply H2.
-      apply H1.
-      apply H0.
-    assert ( claim2 :
-      forall tm : Tm,
-      forall iv : IVar,
-      (forall iv0 : IVar, isFreeIn iv0 tm = true -> iv0 < iv) ->
-      FreshIn iv tm
-    ).
-      intros.
-      unfold FreshIn.
-      assert (isFreeIn iv tm = true -> iv < iv).
-        apply H.
-      destruct (isFreeIn iv tm).
-      assert (iv < iv).
-        apply H0.
-        reflexivity.
-      lia.
-      reflexivity.
-    intros sigma; induction sigma.
-    - intros tm.
-      destruct (claim1 tm) as [iv0].
-      exists iv0.
-      intros.
-      apply claim2.
-      simpl.
-      intros.
-      destruct (Nat.eq_dec iv2 iv).
-      subst.
-      assert (iv0 >= iv).
-        apply g.
-        apply H0.
-      lia.
-      inversion H1.
-    - destruct a as [iv1 tm1].
-      destruct (claim1 tm1) as [iv0].
-      intros.
-      destruct (IHsigma tm) as [iv].
-      exists (max iv iv0).
-      simpl.
-      intros.
-      destruct (Nat.eq_dec iv3 iv1).
-      subst.
-      apply claim2.
-      intros.
-      assert (iv0 >= iv3).
-        apply g.
-        apply H1.
-      lia.
-      apply f.
-      lia.
-      apply H0.
-  Qed.
-
-  Definition funcCHI (sigma : Subst) (tm : Tm) : IVar :=
-    S (proj1_sig (getFreshVariableBound sigma tm))
+    forall sub : Subst,
+    Var iv <> tm ->
+    ~ In iv (map fst sub) ->
+    IsProperSubst sub ->
+    IsProperSubst ((iv, tm) :: sub)
   .
 
-  Lemma funcCHI_gives_fresh_var :
-    forall sigma : Subst,
+  Lemma IsProperSubst_property1 :
+    forall sub : Subst,
+    IsProperSubst sub ->
+    forall iv : IVar,
+    runSubst_Var sub iv = Var iv <-> ~ In iv (map fst sub).
+  Proof.
+    intros sub H.
+    induction H.
+    - intros.
+      unfold runSubst_Var.
+      simpl.
+      tauto.
+    - intros.
+      unfold runSubst_Var.
+      destruct (Nat.eq_dec iv iv0).
+      * subst.
+        constructor.
+        + intro.
+          contradiction H.
+          intuition.
+        + simpl.
+          intro.
+          contradiction H2.
+          left.
+          reflexivity.
+      * simpl.
+        constructor.
+        + intros.
+          intro.
+          destruct H3.
+          contradiction n.
+          apply (proj1 (IHIsProperSubst iv0) H2).
+          apply H3.
+        + intro.
+          assert (~ In iv0 (map fst sub)).
+            intro.
+            apply H2.
+            right.
+            apply H3.
+          assert (runSubst_Var sub iv0 = Var iv0).
+            apply IHIsProperSubst.
+            apply H3.
+          apply H4.
+  Qed.
+
+  Definition FreshInSubst (iv0 : IVar) (sub : Subst) (tm : Tm) : Prop :=
+    forallb (fun iv : IVar => if FreshIn_dec iv0 (runSubst_Var sub iv) then true else false) (getFVs tm) = true
+  .
+
+  Definition getFreeVarBound (tm : Tm) : N :=
+    fold_right max 0 (getFVs tm)
+  .
+
+  Lemma getFreeVarBound_property1 :
+    forall tm : Tm,
+    forall iv : IVar,
+    iv > getFreeVarBound tm ->
+    FreshIn iv tm.
+  Proof.
+    intros tm iv.
+    assert (FreeIn iv tm -> getFreeVarBound tm >= iv).
+      intros.
+      apply (fold_right_max_0_property1 (fun iv0 : IVar => FreeIn iv0 tm)).
+      { intros.
+        apply FreeIn_dec.
+      }
+      { intros.
+        apply getFVs_returns_free_vars.
+        apply H0.
+      }
+      { apply H.
+      }
+      { intro.
+        assert (~ FreeIn iv tm).
+          intro.
+          assert (getFreeVarBound tm >= iv).
+            apply H.
+            apply H1.
+          lia.
+        apply FreshIn_iff.
+        apply H1.
+      }
+  Qed.
+
+  Definition chi (sub : Subst) (tm : Tm) : IVar :=
+    S (fold_right max 0 (map (fun iv0 : IVar => getFreeVarBound (runSubst_Var sub iv0)) (getFVs tm)))
+  .
+
+  Lemma chi_property1 :
+    forall sub : Subst,
     forall tm : Tm,
     forall iv : IVar,
     FreeIn iv tm ->
-    FreshIn (funcCHI sigma tm) (substVar sigma iv).
+    FreshIn (chi sub tm) (runSubst_Var sub iv).
   Proof.
-    intros.
-    unfold funcCHI.
-    destruct (getFreshVariableBound sigma tm) as [bound H0].
-    apply H0.
-    simpl.
-    lia.
-    apply H.
-  Qed.
-
-  Fixpoint substTerm (sigma : Subst) (tm : Tm) : Tm :=
-    match tm with
-    | Var iv => substVar sigma iv
-    | App tm1 tm2 => App (substTerm sigma tm1) (substTerm sigma tm2)
-    | Abs iv tm1 =>
-      let iv' : IVar := funcCHI sigma tm in
-      Abs iv' (substTerm ((iv, Var iv') :: sigma) tm1)
-    end
-  .
-
-  Lemma lemma_1_of_2_6 :
-    forall tm : Tm,
-    forall sigma : Subst,
-    forall iv0 : IVar,
-    FreeIn iv0 tm ->
-    FreshIn (funcCHI sigma tm) (substVar sigma iv0).
-  Proof.
-    cut (
-      forall tm : Tm,
-      forall sigma : Subst,
-      forall iv0 : IVar,
-      FreeIn iv0 tm ->
-      FreshIn (S (proj1_sig (getFreshVariableBound sigma tm))) (substVar sigma iv0)
-    ).
-      intros.
-      apply H.
-      apply H0.
-    intros.
-    inversion H.
+    intros sub tm.
     assert (
-      forall iv0 : IVar,
-      iv0 > proj1_sig (getFreshVariableBound sigma tm) ->
-      forall iv1 : IVar,
-      FreeIn iv1 tm ->
-      FreshIn iv0 (substVar sigma iv1)
-    ).
-      apply (proj2_sig (getFreshVariableBound sigma tm)).
-    apply H0.
-    lia.
-    apply H1.
-  Qed.
-
-  Lemma lemma_2_of_2_6 :
-    forall tm : Tm,
-    FreshIn (funcCHI [] tm) tm.
-  Proof.
-    cut (
-      forall tm0 : Tm,
-      forall iv0 : IVar,
-      FreeIn iv0 tm0 ->
-      iv0 < funcCHI [] tm0
-    ).
-      intros.
-      unfold FreshIn.
-      assert (FreeIn (funcCHI [] tm) tm -> funcCHI [] tm < funcCHI [] tm).
-        apply H.
-      unfold FreeIn in H0.
-      destruct (isFreeIn (funcCHI [] tm) tm).
-      assert (funcCHI [] tm < funcCHI [] tm). 
-        tauto.
-      lia.
-      reflexivity.
-    intros tm.
-    unfold funcCHI.
-    assert (
-      forall iv0 : IVar,
-      iv0 > proj1_sig (getFreshVariableBound [] tm) ->
       forall iv : IVar,
       FreeIn iv tm ->
-      FreshIn iv0 (substVar [] iv)
+      getFreeVarBound (runSubst_Var sub iv) < chi sub tm 
     ).
-      apply (proj2_sig (getFreshVariableBound [] tm)).
+    { intros.
+      unfold chi.
+      cut (
+        fold_right max 0 (map (fun iv0 : IVar => getFreeVarBound (runSubst_Var sub iv0)) (getFVs tm)) >= getFreeVarBound (runSubst_Var sub iv)
+      ).
+        lia.
+      apply (fold_right_max_0_property1 (fun iv' : IVar => In iv' (map (fun iv0 : IVar => getFreeVarBound (runSubst_Var sub iv0)) (getFVs tm)))).
+      { intros.
+        apply In_dec.
+        apply Nat.eq_dec.
+      }
+      { tauto.
+      }
+      { apply in_map_iff.
+        exists iv.
+        constructor.
+        reflexivity.
+        apply getFVs_returns_free_vars.
+        apply H.
+      }
+    }
     intros.
-    cut (~ iv0 >= S (proj1_sig (getFreshVariableBound [] tm))).
-      lia.
-    intro.
-    assert (FreshIn iv0 (substVar [] iv0)).
-    simpl.
+    apply getFreeVarBound_property1.
     apply H.
-    apply H1.
     apply H0.
-    simpl in H2.
-    unfold FreshIn in H2.
-    simpl in H2.
-    destruct (Nat.eq_dec iv0 iv0).
-    inversion H2.
-    contradiction n.
+  Qed.
+
+  Lemma chi_gives_FreshInSubst :
+    forall sub : Subst,
+    forall tm : Tm,
+    FreshInSubst (chi sub tm) sub tm.
+  Proof.
+    intros sub tm.
+    unfold FreshInSubst.
+    cut (
+      forall iv : IVar,
+      In iv (getFVs tm) ->
+      FreshIn (chi sub tm) (runSubst_Var sub iv)
+    ).
+      intros.
+      apply forallb_true_iff.
+      intros iv H0.
+      assert (In iv (getFVs tm) -> FreshIn (chi sub tm) (runSubst_Var sub iv)).
+        apply H.
+      destruct (FreshIn_dec (chi sub tm) (runSubst_Var sub iv)).
+      { reflexivity.
+      }
+      { contradiction n.
+        apply H1.
+        apply H0.
+      }
+    intros.
+    apply chi_property1.
+    apply getFVs_returns_free_vars.
+    apply H.
+  Qed.
+
+  Lemma chi_gives_FreshInSubst_min :
+    forall sub : Subst,
+    forall tm : Tm,
+    forall iv : IVar,
+    iv >= chi sub tm ->
+    FreshInSubst iv sub tm.
+  Proof.
+    assert (
+      forall sub : Subst,
+      forall tm : Tm,
+      forall iv : IVar,
+      (exists iv0 : IVar, FreeIn iv0 tm /\ FreeIn iv (runSubst_Var sub iv0)) ->
+      fold_right max 0 (map (fun iv0 : IVar => S (getFreeVarBound (runSubst_Var sub iv0))) (getFVs tm)) > iv
+    ).
+      intros.
+      apply fold_right_max_0_property2.
+      destruct H as [iv0].
+      destruct H.
+      exists (S (getFreeVarBound (runSubst_Var sub iv0))).
+      constructor.
+      apply in_map_iff.
+      exists iv0.
+      constructor.
+      reflexivity.
+      apply getFVs_returns_free_vars.
+      apply H.
+      cut (~ getFreeVarBound (runSubst_Var sub iv0) < iv).
+        lia.
+      intro.
+      contradiction (proj1 (FreshIn_iff iv (runSubst_Var sub iv0))).
+      apply getFreeVarBound_property1.
+      apply H1.
+    intros.
+    assert (~ (exists iv0 : IVar, FreeIn iv0 tm /\ FreeIn iv (runSubst_Var sub iv0))).
+      intro.
+      assert (fold_right max 0 (map (fun iv0 : IVar => S (getFreeVarBound (runSubst_Var sub iv0))) (getFVs tm)) > iv).
+        apply H.
+        apply H1.
+      assert (
+        chi sub tm >= fold_right max 0 (map (fun iv0 : IVar => S (getFreeVarBound (runSubst_Var sub iv0))) (getFVs tm))
+      ).
+      { unfold chi.
+        induction (getFVs tm).
+        - simpl.
+          lia.
+        - simpl in *.
+          destruct (fold_right max 0 (map (fun iv0 : IVar => S (getFreeVarBound (runSubst_Var sub iv0))) l)).
+          lia.
+          lia.
+      }
+      lia.
+    unfold FreshInSubst.
+    apply forallb_true_iff.
+    intros iv0 H2.
+    assert (~ (if FreshIn_dec iv (runSubst_Var sub iv0) then true else false) = false).
+    { intro.
+      apply H1.
+      exists iv0.
+      constructor.
+      apply getFVs_returns_free_vars.
+      apply H2.
+      destruct (FreshIn_dec iv (runSubst_Var sub iv0)).
+      inversion H3.
+      unfold FreeIn.
+      unfold FreshIn in n.
+      destruct (isFreeIn iv (runSubst_Var sub iv0)).
+      reflexivity.
+      contradiction n.
+    }
+    destruct (FreshIn_dec iv (runSubst_Var sub iv0)).
+    reflexivity.
+    contradiction H3.
     reflexivity.
   Qed.
 
